typeclass/typing/typeclass_typesPropsScript.sml
@@ -1,0 +1,514 @@
+open HolKernel Parse boolLib bossLib BasicProvers;
+open pairTheory arithmeticTheory integerTheory stringTheory optionTheory
+     listTheory alistTheory;
+open mlstringTheory pure_configTheory;
+open typeclass_typesTheory;
+
+val _ = new_theory "typeclass_typesProps";
+
+Theorem type_ind:
+  ∀P.
+    (P (Atom Exception)) ∧
+    (∀s. P (Atom (TypeCons s))) ∧
+    (∀n. P (Atom (VarTypeCons n))) ∧
+    (∀t t'. P t ∧ P t' ⇒ P (Cons t t')) ⇒
+    (∀t. P t)
+Proof
+  ntac 2 strip_tac >>
+  ho_match_mp_tac type_induction >>
+  rw[] >>
+  Cases_on `a` >>
+  simp[]
+QED
+
+Theorem type_full_induction:
+  ∀P.
+    (P (Atom Exception)) ∧
+    (∀n. P (UserType n)) ∧
+    (∀c. P (Atom (CompPrimTy c))) ∧
+    (∀p. P (Atom (PrimTy p))) ∧
+    (∀n. P (Atom (VarTypeCons n))) ∧
+    (∀t t'. P t ∧ P t' ⇒ P (Cons t t')) ⇒
+    (∀t. P t)
+Proof
+  ntac 2 strip_tac >>
+  ho_match_mp_tac type_ind >>
+  rw[] >>
+  Cases_on `s` >>
+  simp[] >>
+  Cases_on `y` >>
+  simp[]
+QED
+
+Theorem type_size_GT_0[simp]:
+  ∀t. 0 < type_size t
+Proof
+  Cases_on `t` >>
+  simp[type_size_def]
+QED
+
+(******************** Functions ********************)
+
+Theorem Functions_APPEND:
+  ∀as bs a.
+    Functions (as ++ bs) a = Functions as (Functions bs a)
+Proof
+  Induct >> rw[Functions_def]
+QED
+
+Theorem Functions_eq_imp:
+  ∀as a bs b.
+    Functions as a = Functions bs b ⇒
+    ∃cs.
+      (as = bs ++ cs ∧ b = Functions cs a) ∨
+      (bs = as ++ cs ∧ a = Functions cs b)
+Proof
+  Induct >> rw[Functions_def] >> csimp[Functions_def]
+  >- (qexists_tac `bs` >> simp[]) >>
+  Cases_on `bs` >> gvs[Functions_def]
+QED
+
+Theorem collect_type_vars_Functions:
+  collect_type_vars (Functions args ret) =
+    BIGUNION (set (MAP collect_type_vars args)) ∪ collect_type_vars ret
+Proof
+  Induct_on `args` >>
+  rw[Functions_def,collect_type_vars_def] >>
+  metis_tac[pred_setTheory.UNION_COMM,
+    pred_setTheory.UNION_ASSOC]
+QED
+
+(******************** Substitutions and shifts ********************)
+
+Theorem shift_db_0[simp]:
+  ∀skip. shift_db skip 0 = I
+Proof
+  simp[FUN_EQ_THM] >>
+  Induct_on `x` using type_ind >>
+  rw[shift_db_def]
+QED
+
+Theorem subst_db_NIL[simp]:
+  ∀n. subst_db n [] = I
+Proof
+  simp[FUN_EQ_THM] >>
+  Induct_on `x` using type_ind >>
+  rw[subst_db_def]
+QED
+
+Theorem subst_db_unchanged:
+  ∀skip ts t n.
+    freetyvars_ok n t ∧
+    n ≤ skip
+  ⇒ subst_db skip ts t = t
+Proof
+  Induct_on `t` using type_ind >>
+  rw[subst_db_def,freetyvars_ok_def] >>
+  metis_tac[]
+QED
+
+Theorem shift_db_unchanged:
+  ∀skip shift t n.
+    freetyvars_ok n t ∧
+    n ≤ skip
+  ⇒ shift_db skip shift t = t
+Proof
+  Induct_on `t` using type_ind >>
+  rw[shift_db_def,freetyvars_ok_def] >>
+  metis_tac[]
+QED
+
+Theorem subst_db_shift_db_unchanged:
+  ∀skip shift t ts m.
+    (m - skip) + LENGTH ts ≤ shift ∧
+    skip ≤ m
+  ⇒ subst_db m ts (shift_db skip shift t) =
+    shift_db skip (shift - LENGTH ts) t
+Proof
+  Induct_on `t` using type_ind >>
+  rw[subst_db_def, shift_db_def]
+QED
+
+Theorem tsubst_tshift:
+  ∀shift t ts m.
+    LENGTH ts ≤ shift
+  ⇒ tsubst ts (tshift shift t) =
+    tshift (shift - LENGTH ts) t
+Proof
+  rw[] >> irule subst_db_shift_db_unchanged >> simp[]
+QED
+
+Theorem subst_db_subst_db:
+  ∀n tsn t m tsm.
+    n ≤ m
+  ⇒ subst_db m tsm (subst_db n tsn t) =
+    subst_db n (MAP (subst_db m tsm) tsn)
+      (subst_db (m + LENGTH tsn) (MAP (shift_db n (LENGTH tsn)) tsm) t)
+Proof
+  Induct_on `t` using type_ind >>
+  rw[subst_db_def, EL_MAP] >>
+  gvs[subst_db_shift_db_unchanged]
+QED
+
+Theorem shift_db_shift_db:
+  ∀m shiftm t n shiftn.
+    n ≤ m
+  ⇒ shift_db (m + shiftn) shiftm (shift_db n shiftn t) =
+    shift_db n shiftn (shift_db m shiftm t)
+Proof
+  recInduct shift_db_ind >> rw[shift_db_def]
+QED
+
+Theorem shift_db_twice:
+  ∀k m ty n. shift_db k n (shift_db k m ty) = shift_db k (n + m) ty
+Proof
+  recInduct shift_db_ind >> rw[shift_db_def]
+QED
+
+Theorem tshift_tshift:
+  ∀t s1 s2.
+    tshift s1 (tshift s2 t) = tshift (s1 + s2) t
+Proof
+  rw[shift_db_twice]
+QED
+
+Theorem subst_db_shift_db_1:
+  ∀n ts t m shift.
+    m ≤ n
+  ⇒ subst_db (n + shift) (MAP (shift_db m shift) ts) (shift_db m shift t) =
+    shift_db m shift (subst_db n ts t)
+Proof
+  recInduct subst_db_ind >> rw[shift_db_def, subst_db_def, EL_MAP]
+QED
+
+Theorem subst_db_shift_db_2:
+  ∀n ts t m shift.
+    n ≤ m
+  ⇒ subst_db n (MAP (shift_db m shift) ts) (shift_db (m + LENGTH ts) shift t) =
+    shift_db m shift (subst_db n ts t)
+Proof
+  recInduct subst_db_ind >> rw[shift_db_def, subst_db_def, EL_MAP]
+QED
+
+(************ tcons_to_type and split_ty_head ************)
+Theorem tcons_to_type_alt:
+  (∀tcons. tcons_to_type tcons [] = Atom $ TypeCons tcons) ∧
+  (∀tcons t1 targs.
+    tcons_to_type tcons (t1::targs) =
+      cons_types (Cons (Atom $ TypeCons tcons) t1) targs)
+Proof
+  rw[tcons_to_type_def] >>
+  simp[Once cons_types_def]
+QED
+
+Theorem cons_types_APPEND:
+   ∀t ts1 ts2.
+     cons_types t (ts1 ++ ts2) = cons_types (cons_types t ts1) ts2
+Proof
+  Induct_on `ts1` >>
+  rw[cons_types_def]
+QED
+
+Theorem cons_types_APPEND_SINGLE:
+  ∀t ts1 t2. cons_types t (ts1 ++ [t2]) = Cons (cons_types t ts1) t2
+Proof
+  simp[cons_types_APPEND,cons_types_def]
+QED
+
+Theorem cons_types_SNOC:
+  ∀t ts1 t2. cons_types t (SNOC t2 ts1) = Cons (cons_types t ts1) t2
+Proof
+  simp[cons_types_APPEND_SINGLE,SNOC_APPEND]
+QED
+
+Theorem tcons_to_type_APPEND:
+  tcons_to_type tcons (ts1 ++ ts2) = cons_types (tcons_to_type tcons ts1) ts2
+Proof
+  simp[tcons_to_type_def,cons_types_APPEND]
+QED
+
+Theorem tcons_to_type_SNOC:
+  tcons_to_type tcons (SNOC t ts1) = Cons (tcons_to_type tcons ts1) t
+Proof
+  simp[tcons_to_type_APPEND,SNOC_APPEND,cons_types_def]
+QED
+
+Theorem type_size_cons_types:
+  (∀t targs. type_size (cons_types t []) = type_size t) ∧
+  (∀t t' targs. type_size t <
+    type_size (cons_types t (t'::targs))) ∧
+  (∀t t' targs.
+    MEM t targs ⇒
+    type_size t < type_size (cons_types t' targs))
+Proof
+  conj_tac >- simp[cons_types_def] >>
+  conj_tac >- (
+    Induct_on `targs` >>
+    fs[cons_types_def,type_size_def] >>
+    rw[] >>
+    irule LESS_EQ_LESS_TRANS >>
+    first_x_assum $ irule_at (Pos hd) >>
+    simp[type_size_def]) >>
+  Induct_on `targs` using SNOC_INDUCT >>
+  rw[cons_types_SNOC,type_size_def]
+  >- rw[] >>
+  irule arithmeticTheory.LESS_LESS_EQ_TRANS >>
+  first_x_assum $ drule_then $ irule_at (Pos hd) >>
+  qexists_tac `t'` >>
+  DECIDE_TAC
+QED
+
+Theorem type_size_tcons_to_type:
+  ∀t targs tcons.
+  MEM t targs ⇒
+  type_size t < type_size (tcons_to_type tcons targs)
+Proof
+  rw[tcons_to_type_def,type_size_cons_types]
+QED
+
+Theorem tcons_to_type_NEQ_TypeVar:
+  ∀v tcons targs. tcons_to_type tcons targs ≠ TypeVar v
+Proof
+  simp[tcons_to_type_def] >>
+  Cases_on `targs` using SNOC_CASES >>
+  simp[cons_types_def,cons_types_SNOC]
+QED
+
+Theorem ty_args_aux_SNOC:
+  ∀t t1 t2 l. t = Cons t1 t2 ⇒ ty_args_aux t l = ty_args_aux t1 [] ++ (t2::l)
+Proof
+  Induct_on `t` >>
+  rw[] >>
+  Cases_on `t` >>
+  gvs[ty_args_aux_def]
+QED
+
+Theorem ty_args_SNOC:
+  ty_args (Cons t1 t2) = SNOC t2 (ty_args t1)
+Proof
+  simp[ty_args_def,ty_args_aux_SNOC]
+QED
+
+Theorem ty_args_alt:
+  (∀t1 t2. ty_args (Cons t1 t2) = SNOC t2 (ty_args t1)) ∧
+  (∀x. ty_args (Atom x) = [])
+Proof
+  simp[ty_args_SNOC] >> simp[ty_args_def,ty_args_aux_def]
+QED
+
+Theorem head_ty_cons_eq_head_ty:
+  ∀t c. (head_ty_cons t = SOME c) ⇔ (head_ty t = TypeCons c)
+Proof
+  Induct_on `t` using type_ind >>
+  simp[head_ty_cons_def,head_ty_def]
+QED
+
+Theorem split_ty_cons_aux_eq_split_ty_aux:
+  ∀t l c targs.
+    (split_ty_cons_aux t l = SOME (c,targs)) ⇔
+    (split_ty_aux t l = (TypeCons c,targs))
+Proof
+  Induct_on `t` using type_ind >>
+  simp[split_ty_cons_aux_def,split_ty_aux_def]
+QED
+
+Theorem split_ty_cons_eq_split_ty:
+  ∀t c targs.
+    (split_ty_cons t = SOME (c,targs)) ⇔
+    (split_ty t = (TypeCons c,targs))
+Proof
+  simp[split_ty_cons_def,split_ty_def,
+    split_ty_cons_aux_eq_split_ty_aux]
+QED
+
+Theorem split_ty_aux_thm:
+  ∀t l c targs.
+    split_ty_aux t l = (c,targs) ⇔
+    (head_ty t = c ∧ ty_args_aux t l = targs)
+Proof
+  Induct_on `t` using type_ind >>
+  rw[split_ty_aux_def,head_ty_def,ty_args_aux_def]
+QED
+
+Theorem split_ty_thm:
+  ∀t c targs.
+    split_ty t = (c,targs) ⇔
+    (head_ty t = c ∧ ty_args t = targs)
+Proof
+  simp[split_ty_def,ty_args_def,split_ty_aux_thm]
+QED
+
+Theorem split_ty_cons_aux_thm:
+  ∀t l tc targs.
+    split_ty_cons_aux t l = SOME (tc,targs) ⇔
+    (head_ty_cons t = SOME tc ∧ ty_args_aux t l = targs)
+Proof
+  rw[split_ty_cons_aux_eq_split_ty_aux,
+    head_ty_cons_eq_head_ty,split_ty_aux_thm]
+QED
+
+Theorem split_ty_cons_thm:
+  ∀t tc targs.
+    split_ty_cons t = SOME (tc,targs) ⇔
+    (head_ty_cons t = SOME tc ∧ ty_args t = targs)
+Proof
+  simp[split_ty_cons_eq_split_ty,head_ty_cons_eq_head_ty,
+    split_ty_thm]
+QED
+
+Theorem head_ty_cons_types:
+  ∀t targs. head_ty (cons_types t targs) = head_ty t
+Proof
+  Induct_on `targs` >>
+  rw[head_ty_def,cons_types_def]
+QED
+
+Theorem head_ty_cons_cons_types:
+  ∀t targs. head_ty_cons (cons_types t targs) = head_ty_cons t
+Proof
+  Induct_on `targs` >>
+  rw[head_ty_cons_def,cons_types_def]
+QED
+
+Theorem ty_args_cons_types:
+  ∀t targs. ty_args (cons_types t targs) = ty_args t ++ targs
+Proof
+  Induct_on `targs` >>
+  rw[cons_types_def,ty_args_alt]
+QED
+
+Theorem split_ty_cons_types:
+  ∀at targs. split_ty (cons_types (Atom at) targs) = (at, targs)
+Proof
+  Induct_on `targs` using SNOC_INDUCT >>
+  fs[cons_types_def,split_ty_thm] >>
+  rw[head_ty_def,ty_args_alt,cons_types_def,
+    SNOC_APPEND,cons_types_APPEND]
+QED
+
+Theorem split_ty_cons_tcons_to_type:
+  split_ty_cons (tcons_to_type tcons targs) = SOME (tcons, targs)
+Proof
+  simp[split_ty_cons_eq_split_ty,tcons_to_type_def,
+    split_ty_cons_types]
+QED
+
+Theorem cons_types_head_ty_ty_args:
+  cons_types (Atom $ head_ty t) (ty_args t) = t
+Proof
+  Induct_on `t` using type_ind >>
+  fs[cons_types_def,cons_types_SNOC,
+    head_ty_def,ty_args_alt]
+QED
+
+Theorem tcons_to_type_split_ty_cons:
+  ∀t tcons targs.
+    split_ty_cons t = SOME (tcons,targs) ⇒
+    tcons_to_type tcons targs = t
+Proof
+  rw[split_ty_cons_thm,tcons_to_type_def,
+    head_ty_cons_eq_head_ty] >>
+  metis_tac[cons_types_head_ty_ty_args]
+QED
+
+Theorem subst_db_cons_types:
+  ∀n ts thd targs.
+    subst_db n ts (cons_types thd targs) =
+    cons_types (subst_db n ts thd) $ MAP (subst_db n ts) targs
+Proof
+  Induct_on `targs` >>
+  rw[cons_types_def,subst_db_def]
+QED
+
+Theorem subst_db_tcons_to_type:
+  ∀skip ts tcons targs.
+  subst_db skip ts (tcons_to_type tcons targs) =
+    tcons_to_type tcons $ MAP (subst_db skip ts) targs
+Proof
+  rw[tcons_to_type_def,subst_db_cons_types,subst_db_def]
+QED
+
+Theorem shift_db_cons_types:
+  ∀skip n thd targs.
+    shift_db skip n (cons_types thd targs) =
+    cons_types (shift_db skip n thd) $ MAP (shift_db skip n) targs
+Proof
+  Induct_on `targs` >>
+  rw[cons_types_def,shift_db_def]
+QED
+
+Theorem shift_db_tcons_to_type:
+  ∀skip n tcons targs.
+  shift_db skip n (tcons_to_type tcons targs) =
+    tcons_to_type tcons $ MAP (shift_db skip n) targs
+Proof
+  rw[tcons_to_type_def,shift_db_cons_types,shift_db_def]
+QED
+
+(******************** Properties of types ********************)
+
+Theorem freetyvars_ok_mono:
+  ∀n t m.
+    freetyvars_ok n t ∧
+    n ≤ m
+  ⇒ freetyvars_ok m t
+Proof
+  recInduct freetyvars_ok_ind >> rw[freetyvars_ok_def]
+QED
+
+Theorem freetyvars_ok_subst_db:
+  ∀skip ts t n.
+    freetyvars_ok (n + LENGTH ts) t ∧
+    EVERY (freetyvars_ok n) ts ∧
+    skip ≤ n
+  ⇒ freetyvars_ok n (subst_db skip ts t)
+Proof
+  recInduct subst_db_ind >>
+  rw[subst_db_def, freetyvars_ok_def] >>
+  gvs[EVERY_MEM, MEM_EL, PULL_EXISTS]
+QED
+
+Theorem freetyvars_ok_tsubst:
+  ∀ts t n.
+    freetyvars_ok (n + LENGTH ts) t ∧
+    EVERY (freetyvars_ok n) ts
+  ⇒ freetyvars_ok n (tsubst ts t)
+Proof
+  rw[] >> irule freetyvars_ok_subst_db >> simp[]
+QED
+
+Theorem freetyvars_ok_shift_db:
+  ∀skip shift t n.
+    freetyvars_ok n t
+  ⇒ freetyvars_ok (n + shift) (shift_db skip shift t)
+Proof
+  recInduct shift_db_ind >>
+  rw[shift_db_def, freetyvars_ok_def]
+QED
+
+Theorem freetyvars_ok_Functions:
+  ∀ats rt db.
+    freetyvars_ok db (Functions ats rt) ⇔
+    EVERY (freetyvars_ok db) ats ∧
+    freetyvars_ok db rt
+Proof
+  Induct >> rw[Functions_def, freetyvars_ok_def] >> eq_tac >> rw[]
+QED
+
+Theorem subst_db_Functions:
+  ∀ats rt n ts.
+    subst_db n ts (Functions ats rt) =
+    Functions (MAP (subst_db n ts) ats) (subst_db n ts rt)
+Proof
+  Induct >> rw[Functions_def, subst_db_def]
+QED
+
+Theorem shift_db_Functions:
+  ∀ats rt skip shift.
+    shift_db skip shift (Functions ats rt) =
+    Functions (MAP (shift_db skip shift) ats) (shift_db skip shift rt)
+Proof
+  Induct >> rw[Functions_def, shift_db_def]
+QED
+
+val _ = export_theory();
