typeclass/typing/typeclass_typingProofScript.sml
@@ -1,0 +1,16 @@
+open HolKernel Parse boolLib bossLib BasicProvers dep_rewrite;
+open pairTheory arithmeticTheory integerTheory stringTheory optionTheory miscTheory;
+open listTheory alistTheory relationTheory set_relationTheory pred_setTheory;
+open typeclass_typesTheory pure_cexpTheory;
+open pure_tcexpTheory pure_tcexp_typingTheory
+pure_tcexp_typingPropsTheory;
+open typeclass_texpTheory;
+open typeclass_kindCheckTheory pure_configTheory;
+open monadsyntax;
+
+val _ = monadsyntax.enable_monadsyntax();
+val _ = monadsyntax.enable_monad "option";
+
+val _ = new_theory "typeclass_typingProof";
+
+val _ = export_theory();
